src/program_proof/tulip/invariance/commit.v
@@ -1,0 +1,859 @@
+From Perennial.program_proof.tulip Require Import prelude.
+
+Lemma lookup_resm_to_tmods_Some resm ts wrs :
+  resm_to_tmods resm !! ts = Some wrs ↔
+  resm !! ts = Some (ResCommitted wrs).
+Proof.
+  rewrite /resm_to_tmods lookup_omap.
+  destruct (resm !! ts) as [res |] eqn:Hres; last done.
+  split; intros Hresm.
+  - by destruct res as [wrsx |] eqn:Hwrsx; first inv Hresm.
+  - by rewrite Hresm /=.
+Qed.
+
+Lemma lookup_resm_to_tmods_None resm ts :
+  resm_to_tmods resm !! ts = None ↔
+  resm !! ts = None ∨ resm !! ts = Some ResAborted.
+Proof.
+  split; intros Hresm.
+  - destruct (resm !! ts) as [res |] eqn:Hres; last by left.
+    destruct res as [wrs |]; last by right.
+    exfalso.
+    by rewrite /resm_to_tmods lookup_omap Hres in Hresm.
+  - rewrite /resm_to_tmods lookup_omap.
+    by destruct Hresm as [Hresm | Hresm]; rewrite Hresm.
+Qed.
+
+Lemma ext_by_cmtd_length repl cmtd kmodc ts :
+  ts ≠ O ->
+  kmodc !! ts = None ->
+  ext_by_cmtd repl cmtd kmodc ts ->
+  (length cmtd ≤ ts)%nat.
+Proof.
+  intros Hnz Hnone Hext.
+  rewrite /ext_by_cmtd Hnone in Hext.
+  destruct Hext as [-> Hlen].
+  by specialize (Hlen Hnz).
+Qed.
+
+Lemma no_commit_head_commit future ts wrs :
+  no_commit_abort future ts ->
+  head_commit future ts wrs ->
+  False.
+Proof.
+  intros [_ Hnc] Hhc.
+  specialize (Hnc wrs).
+  by apply head_Some_elem_of in Hhc.
+Qed.
+
+Lemma first_abort_head_commit future ts wrs :
+  first_abort future ts ->
+  head_commit future ts wrs ->
+  False.
+Proof.
+  intros (lp & ls & (Happ & [_ Hnc] & Hhead)) Hhc.
+  destruct (decide (lp = [])) as [-> | Hnnil].
+  { rewrite Happ /= /head_commit Hhead in Hhc. by inv Hhc. }
+  assert (Hlp : ActCommit ts wrs ∈ lp).
+  { apply head_Some_elem_of.
+    rewrite (head_prefix _ future); [done | apply Hnnil |].
+    rewrite Happ.
+    by apply prefix_app_r.
+  }
+  by specialize (Hnc _ Hlp).
+Qed.
+
+Lemma first_commit_head_commit future lp ls ts wrs wrshd :
+  first_commit future lp ls ts wrs ->
+  head_commit future ts wrshd ->
+  wrshd = wrs.
+Proof.
+  intros (Happ & [_ Hnc] & Hhead) Hhc.
+  destruct lp as [| x l]; last first.
+  { rewrite Happ /head_commit /= in Hhc.
+    inv Hhc.
+    specialize (Hnc wrshd).
+    set_solver.
+  }
+  rewrite Happ /= /head_commit Hhead in Hhc.
+  by inv Hhc.
+Qed.
+
+Lemma first_commit_compatible_head_commit future ts tshd wrs wrshd :
+  first_commit_compatible future ts wrs ->
+  head_commit future tshd wrshd ->
+  dom wrs ∩ dom wrshd ≠ ∅ ->
+  (tshd ≤ ts)%nat.
+Proof.
+  intros (lp & ls & (Happ & _ & Hhead) & Hcomp) Hhc Hnempty.
+  destruct (decide (lp = [])) as [-> | Hnnil].
+  { rewrite Happ /= /head_commit Hhead in Hhc. by inv Hhc. }
+  assert (Hlp : ActCommit tshd wrshd ∈ lp).
+  { apply head_Some_elem_of.
+    rewrite (head_prefix _ future); [done | apply Hnnil |].
+    rewrite Happ.
+    by apply prefix_app_r.
+  }
+  rewrite /compatible_all Forall_forall in Hcomp.
+  specialize (Hcomp _ Hlp).
+  destruct Hcomp; [lia | contradiction].
+Qed.
+
+Lemma first_commit_incompatible_head_commit past future ts wrs wrshd :
+  first_commit_incompatible past future ts wrs ->
+  head_commit future ts wrshd ->
+  wrshd = wrs ∧ ∃ a, a ∈ past ∧ not (compatible ts wrs a).
+Proof.
+  intros (lp & ls & (Happ & [_ Hnc] & Hhead) & Hincomp) Hhc.
+  destruct lp as [| x l]; last first.
+  { rewrite Happ /head_commit /= in Hhc.
+    inv Hhc.
+    specialize (Hnc wrshd).
+    set_solver.
+  }
+  rewrite Happ /= /head_commit Hhead in Hhc.
+  inv Hhc.
+  split; first done.
+  by rewrite app_nil_r /incompatible_exists Exists_exists in Hincomp.
+Qed.
+
+Lemma first_abort_inv_commit future ts tshd wrshd :
+  head_commit future tshd wrshd ->
+  first_abort future ts ->
+  first_abort (tail future) ts.
+Proof.
+  intros Hhead Hfa.
+  by unshelve eapply (first_abort_inv_tail_future _ _ _ _ Hhead Hfa).
+Qed.
+
+Lemma first_commit_compatible_inv_commit future ts tshd wrs wrshd :
+  ts ≠ tshd ->
+  head_commit future tshd wrshd ->
+  first_commit_compatible future ts wrs ->
+  first_commit_compatible (tail future) ts wrs.
+Proof.
+  intros Hne Hhead Hfci.
+  unshelve eapply (first_commit_compatible_inv_tail_future _ _ _ _ _ Hhead).
+  { intros Heq. inv Heq. }
+  done.
+Qed.
+
+Lemma first_commit_incompatible_inv_commit past future ts tshd wrs wrshd :
+  ts ≠ tshd ->
+  head_commit future tshd wrshd ->
+  first_commit_incompatible past future ts wrs ->
+  first_commit_incompatible (past ++ [ActCommit tshd wrshd]) (tail future) ts wrs.
+Proof.
+  intros Hne Hhead Hfci.
+  apply first_commit_incompatible_inv_snoc_past_tail_future.
+  { intros Heq. inv Heq. }
+  { done. }
+  done.
+Qed.
+
+Lemma conflict_free_head_commit_eq future tmods ts wrs wrshd :
+  conflict_free future tmods ->
+  head_commit future ts wrshd ->
+  tmods !! ts = Some wrs ->
+  wrshd = wrs.
+Proof.
+  intros Hcf Hhead Hwrs.
+  specialize (Hcf _ _ Hwrs). simpl in Hcf.
+  destruct Hcf as (lp & ls & Hfc & _).
+  by eapply first_commit_head_commit.
+Qed.
+
+Lemma conflict_free_head_commit_le_all future tmodcs ts wrs :
+  conflict_free future tmodcs ->
+  head_commit future ts wrs ->
+  set_Forall (λ k, le_all ts (dom (vslice tmodcs k))) (dom wrs).
+Proof.
+  intros Hcf Hhead k Hk tsx Htsx.
+  rewrite elem_of_dom in Htsx.
+  destruct Htsx as [v Hv].
+  rewrite lookup_vslice /dual_lookup in Hv.
+  destruct (tmodcs !! tsx) as [wrsx |] eqn:Hwrsx; rewrite Hwrsx in Hv; last done.
+  specialize (Hcf _ _ Hwrsx). simpl in Hcf.
+  eapply first_commit_compatible_head_commit; [done | done |].
+  apply elem_of_dom_2 in Hv.
+  set_solver.
+Qed.
+
+Lemma conflict_free_inv_commit_committed ts wrs future tmodcs :
+  tmodcs !! ts = None ->
+  head_commit future ts wrs ->
+  conflict_free future tmodcs ->
+  conflict_free (tail future) tmodcs.
+Proof.
+  intros Hnone Hhead Hcf.
+  intros tsx wrsx Hlookup.
+  specialize (Hcf _ _ Hlookup). simpl in Hcf.
+  eapply first_commit_compatible_inv_commit; [| apply Hhead | apply Hcf].
+  intros Heq. subst tsx.
+  by rewrite Hnone in Hlookup.
+Qed.
+
+Lemma conflict_free_inv_commit ts wrs future tmodcs :
+  head_commit future ts wrs ->
+  conflict_free future tmodcs ->
+  conflict_free (tail future) (delete ts tmodcs).
+Proof.
+  intros Hhead Hcf.
+  intros tsx wrsx Hlookup.
+  rewrite lookup_delete_Some in Hlookup.
+  destruct Hlookup as [Hne Hlookup].
+  specialize (Hcf _ _ Hlookup). simpl in Hcf.
+  eapply first_commit_compatible_inv_commit; [done | apply Hhead | apply Hcf].
+Qed.
+
+Lemma conflict_past_inv_commit ts wrs past future tmodas :
+  ts ∉ dom tmodas ->
+  head_commit future ts wrs ->
+  conflict_past past future tmodas ->
+  conflict_past (past ++ [ActCommit ts wrs]) (tail future) tmodas.
+Proof.
+  intros Hnoin Hhead Hcp.
+  intros tsx form Hlookup.
+  specialize (Hcp _ _ Hlookup). simpl in Hcp.
+  apply elem_of_dom_2 in Hlookup.
+  assert (Hne : ts ≠ tsx) by set_solver.
+  rewrite /conflict_cases in Hcp.
+  destruct form as [| | wrsx | wrsx]; simpl.
+  - by apply no_commit_abort_inv_tail_future.
+  - by eapply first_abort_inv_commit.
+  - by apply first_commit_incompatible_inv_commit.
+  - by eapply first_commit_compatible_inv_commit.
+Qed.
+
+Lemma cmtxn_in_past_inv_commit past resm ts wrs :
+  cmtxn_in_past past resm ->
+  cmtxn_in_past (past ++ [ActCommit ts wrs]) (<[ts := ResCommitted wrs]> resm).
+Proof.
+  intros Hcmtxn t m Htm.
+  rewrite resm_to_tmods_insert_committed in Htm.
+  destruct (decide (ts = t)) as [-> | Hne].
+  { rewrite lookup_insert in Htm. inv Htm. set_solver. }
+  rewrite lookup_insert_ne in Htm; last done.
+  specialize (Hcmtxn _ _ Htm).
+  set_solver.
+Qed.
+
+Lemma cmtxn_in_past_inv_commit_committed past resm ts wrs :
+  resm !! ts = Some (ResCommitted wrs) ->
+  cmtxn_in_past past resm ->
+  cmtxn_in_past (past ++ [ActCommit ts wrs]) resm.
+Proof.
+  intros Hsome Hcmtxn t m Htm.
+  specialize (Hcmtxn _ _ Htm).
+  set_solver.
+Qed.
+
+Lemma ext_by_lnrz_inv_commit ts v cmtd lnrz kmodl :
+  kmodl !! ts = Some v ->
+  le_all ts (dom kmodl) ->
+  ext_by_lnrz cmtd lnrz kmodl ->
+  ext_by_lnrz (last_extend ts cmtd ++ [v]) lnrz (delete ts kmodl).
+Proof.
+  intros Hv Hles Hext.
+  destruct Hext as (vlast & Hprefix & Hlast & Hlen & Hext).
+  (* Obtain [length cmtd ≤ ts < length lnrz]. *)
+  apply elem_of_dom_2 in Hv as Hts.
+  apply Hlen in Hts.
+  exists v.
+  split.
+  { (* Re-establish prefix. *)
+    apply prefix_pointwise.
+    intros i Hi.
+    (* Obtain [i < S ts]. *)
+    rewrite last_length last_extend_length_eq_n in Hi; [| set_solver | lia].
+    destruct (decide (i < length cmtd)%nat) as [Hilt | Hige].
+    { (* Case: before extension [i < length cmtd]. *)
+      rewrite /last_extend Hlast /extend.
+      rewrite -app_assoc lookup_app_l; last done.
+      by apply prefix_lookup_lt.
+    }
+    rewrite Nat.nlt_ge in Hige.
+    assert (is_Some (lnrz !! i)) as [u Hu].
+    { rewrite lookup_lt_is_Some. lia. }
+    assert (Higeweak : (pred (length cmtd) ≤ i)%nat) by lia.
+    rewrite Hu.
+    destruct (decide (i < ts)%nat) as [Hits | Hits].
+    { (* Case: read-extension [i < ts]. *)
+      specialize (Hext _ _ Higeweak Hu).
+      rewrite lookup_app_l; last first.
+      { by rewrite last_extend_length_eq_n; [| set_solver | lia]. }
+      rewrite /last_extend Hlast /extend.
+      rewrite lookup_app_r; last done.
+      rewrite lookup_replicate.
+      split; last lia.
+      rewrite -Hext.
+      apply prev_dbval_lt_all.
+      intros n Hn.
+      (* Obtain [ts ≤ n]. *)
+      specialize (Hles _ Hn). simpl in Hles.
+      (* Prove [i < n] by [i < ts] and [ts ≤ n]. *)
+      lia.
+    }
+    (* Case: write-extension [i = ts]. *)
+    assert (i = ts) by lia. clear Hits Hi. subst i.
+    rewrite lookup_snoc_Some. right.
+    split.
+    { by rewrite last_extend_length_eq_n; [| set_solver | lia]. }
+    specialize (Hext _ _ Higeweak Hu).
+    by rewrite (prev_dbval_lookup _ _ _ _ Hv) in Hext.
+  }
+  split.
+  { (* Re-establish last. *)
+    by rewrite last_snoc.
+  }
+  split.
+  { (* Re-establish len. *)
+    intros n Hn.
+    rewrite last_length last_extend_length_eq_n; [| set_solver | lia].
+    rewrite dom_delete_L elem_of_difference not_elem_of_singleton in Hn.
+    destruct Hn as [Hin Hne].
+    specialize (Hlen _ Hin). simpl in Hlen.
+    specialize (Hles _ Hin). simpl in Hles.
+    lia.
+  }
+  (* Re-establish ext. *)
+  intros t u Ht Hu.
+  rewrite last_length last_extend_length_eq_n in Ht; [| set_solver | lia].
+  erewrite prev_dbval_delete; [| lia | done | done].
+  apply Hext; [lia | done].
+Qed.
+
+Lemma ext_by_cmtd_inv_commit repl cmtd kmodc ts v :
+  ts ≠ O ->
+  kmodc !! ts = None ->
+  ext_by_cmtd repl cmtd kmodc ts ->
+  ext_by_cmtd repl (last_extend ts cmtd ++ [v]) (<[ts := v]> kmodc) ts.
+Proof.
+  intros Hnz Hts Hext.
+  rewrite /ext_by_cmtd Hts in Hext.
+  destruct Hext as [-> Hlen].
+  by rewrite /ext_by_cmtd lookup_insert.
+Qed.
+
+Section inv.
+  Context `{!tulip_ghostG Σ}.
+
+  Lemma keys_inv_prepared_at_ts γ resm wrs ts :
+    resm !! ts = None ->
+    all_prepared γ ts wrs -∗
+    ([∗ set] key ∈ dom wrs, key_inv γ key) -∗
+    own_txn_resm γ resm -∗
+    ([∗ set] gid ∈ gids_all, group_inv γ gid) -∗
+    ([∗ set] key ∈ dom wrs, key_inv_with_tsprep γ key ts) ∗
+    own_txn_resm γ resm ∗
+    ([∗ set] gid ∈ gids_all, group_inv γ gid).
+  Proof.
+    iIntros (Hnone) "#Hpreps Hkeys Hresm Hgroups".
+    iApply (big_sepS_impl_res with "Hkeys [Hresm Hgroups]").
+    { iFrame. }
+    iIntros (k Hk) "!> Hkey [Hresm Hgroups]".
+    iDestruct "Hpreps" as "[Hwrs Hpreps]".
+    set gid := key_to_group k.
+    iDestruct (big_sepS_elem_of _ _ gid with "Hpreps") as "Hprep".
+    { by apply elem_of_key_to_group_ptgroups. }
+    iDestruct (big_sepS_elem_of_acc _ _ gid with "Hgroups") as "[Hgroup HgroupsC]".
+    { apply elem_of_key_to_group. }
+    do 2 iNamed "Hgroup".
+    iDestruct (group_prep_lookup with "Hpm Hprep") as %Hp.
+    assert (is_Some (stm !! ts)) as [res Hres].
+    { rewrite -elem_of_dom. apply elem_of_dom_2 in Hp. set_solver. }
+    destruct res as [pwrs | |]; last first.
+    { (* Case: Txn [ts] has already aborted. Contradiction. *)
+      iDestruct (big_sepM_lookup with "Hsafestm") as "Habt"; first apply Hres.
+      iDestruct (txn_res_lookup with "Hresm Habt") as %Habt.
+      congruence.
+    }
+    { (* Case: Txn [ts] has already committed. Contradiction. *)
+      iDestruct (big_sepM_lookup with "Hsafestm") as "Hcmt"; first apply Hres.
+      iDestruct "Hcmt" as (wrs') "Hcmt".
+      iDestruct (txn_res_lookup with "Hresm Hcmt") as %Hcmt.
+      congruence.
+    }
+    iDestruct (big_sepM_lookup with "Hsafestm") as "Hpreped"; first apply Hres.
+    iDestruct "Hpreped" as "[Hpreped Hsafep]".
+    iDestruct "Hsafep" as (wrs') "(Hwrs' & _ & %Hvw & %Hne & %Hpwrs)".
+    iDestruct (txn_wrs_agree with "Hwrs Hwrs'") as %->.
+    assert (Hinpwrs : k ∈ dom pwrs).
+    { rewrite Hpwrs /wrs_group.
+      assert (Hgoal : k ∈ filter (λ k, key_to_group k = gid) (dom wrs)).
+      { by rewrite elem_of_filter. }
+      by rewrite filter_dom_L in Hgoal.
+    }
+    (* From [prepared_impl_locked] we obtain a locked [tpl] associated with [k]. *)
+    destruct (Hpil _ _ _ Hres Hinpwrs) as (tpl & Htpl & Hlocked).
+    (* Take [tuple_repl_half] from [Hrepls]. *)
+    iDestruct (big_sepM_lookup_acc _ _ k tpl with "Hrepls") as "[[Hhist Hts] HreplsC]".
+    { by rewrite /tpls_group map_lookup_filter_Some. }
+    iDestruct (key_inv_expose_tsprep with "Hkey") as (tsprep) "Hkey".
+    (* Finally, deduce [tsprep = ts]. *)
+    iAssert (⌜tsprep = ts⌝)%I as %->.
+    { do 2 iNamed "Hkey".
+      iDestruct (repl_ts_agree with "Htsprep Hts") as %Heq.
+      by rewrite Hlocked in Heq.
+    }
+    iDestruct ("HreplsC" with "[$Hhist $Hts]") as "Hrepls".
+    iDestruct ("HgroupsC" with "[-Hresm Hkey]") as "Hgroups".
+    { iFrame "∗ # %". }
+    iFrame.
+  Qed.
+
+  Definition key_inv_after_commit
+    γ (key : dbkey) (tsprep : nat) (kmodl kmodc : dbkmod) : iProp Σ :=
+    ∃ v, let kmodl' := delete tsprep kmodl in
+         let kmodc' := <[tsprep := v]> kmodc in
+         key_inv_with_tsprep_no_kmodl_no_kmodc γ key tsprep kmodl' kmodc' ∗
+         ⌜kmodl !! tsprep = Some v⌝.
+
+  Lemma key_inv_commit γ kmodl kmodc ts k v :
+    ts ≠ O ->
+    le_all ts (dom kmodl) ->
+    kmodl !! ts = Some v ->
+    kmodc !! ts = None ->
+    key_inv_with_tsprep_no_kmodl_no_kmodc γ k ts kmodl kmodc ==∗
+    key_inv_with_tsprep_no_kmodl_no_kmodc γ k ts (delete ts kmodl) (<[ts:=v]> kmodc) ∗
+    is_cmtd_hist_length_lb γ k (S ts).
+  Proof.
+    iIntros (Hnz Hles Hkmodl Hkmodc) "Hkey".
+    do 2 iNamed "Hkey".
+    pose proof (ext_by_lnrz_inv_commit _ _ _ _ _ Hkmodl Hles Hdiffl) as Hdiffl'.
+    pose proof (ext_by_cmtd_inv_commit _ _ _ _ v Hnz Hkmodc Hdiffc) as Hdiffc'.
+    set cmtd' := last_extend _ _ ++ _ in Hdiffl'.
+    iMod (cmtd_hist_update cmtd' with "Hcmtd") as "Hcmtd".
+    { apply prefix_app_r, last_extend_prefix. }
+    iDestruct (cmtd_hist_witness with "Hcmtd") as "#Hlb".
+    iFrame "∗ # %".
+    iPureIntro.
+    split; first by rewrite lookup_insert_ne.
+    subst cmtd'.
+    pose proof (ext_by_lnrz_not_nil _ _ _ Hdiffl) as Hnnil.
+    apply (last_extend_length ts) in Hnnil.
+    rewrite length_app /=.
+    lia.
+  Qed.
+
+  Lemma keys_inv_commit γ kmodls kmodcs ts :
+    ts ≠ O ->
+    map_Forall (λ _ kmodl, le_all ts (dom kmodl)) kmodls ->
+    map_Forall (λ _ kmodl, is_Some (kmodl !! ts)) kmodls ->
+    map_Forall (λ _ kmodc, kmodc !! ts = None) kmodcs ->
+    ([∗ map] key ↦ kmodl;kmodc ∈ kmodls;kmodcs,
+       key_inv_with_tsprep_no_kmodl_no_kmodc γ key ts kmodl kmodc) ==∗
+    ([∗ map] key ↦ kmodl;kmodc ∈ kmodls;kmodcs,
+       key_inv_after_commit γ key ts kmodl kmodc ∗ is_cmtd_hist_length_lb γ key (S ts)).
+  Proof.
+    iIntros (Hnz Hles Hkmodls Hkmodcs) "Hkeys".
+    iApply big_sepM2_bupd.
+    iApply (big_sepM2_impl with "Hkeys").
+    iIntros (k kmodl kmodc Hkmodl Hkmodc) "!> Hkey".
+    specialize (Hkmodls _ _ Hkmodl). simpl in Hkmodls.
+    specialize (Hles _ _ Hkmodl). simpl in Hles.
+    specialize (Hkmodcs _ _ Hkmodc). simpl in Hkmodcs.
+    destruct Hkmodls as [v Hv].
+    iMod (key_inv_commit with "Hkey") as "[Hkey #Hlb]"; try done.
+    iModIntro.
+    iSplit; last iFrame "Hlb".
+    iExists v.
+    by iFrame "%".
+  Qed.
+
+  Lemma partitioned_tids_close {γ} tids tmodcs tmodas resm :
+    let wcmts := dom tmodcs in
+    let wabts := dom tmodas in
+    let cmts := dom (resm_to_tmods resm) in
+    set_Forall (λ tid : nat, tid ∈ dom resm ∨ tid ∈ wabts ∨ tid ∈ wcmts) tids ->
+    ([∗ set] tid ∈ wcmts, own_excl_tid γ tid) -∗
+    ([∗ set] tid ∈ wabts, own_excl_tid γ tid) -∗
+    ([∗ set] tid ∈ cmts, own_excl_tid γ tid) -∗
+    partitioned_tids γ tids tmodcs tmodas resm.
+  Proof. iIntros (wcmts wabts cmts Hfate) "Hwcmts Habts Hcmts". iFrame "∗ %". Qed.
+
+  Lemma txnsys_inv_commit γ tid wrs future :
+    head_commit future tid wrs ->
+    is_lnrz_tid γ tid -∗
+    all_prepared γ tid wrs -∗
+    txnsys_inv_no_future γ future -∗
+    ([∗ set] gid ∈ gids_all, group_inv γ gid) -∗
+    ([∗ set] key ∈ keys_all, key_inv γ key) ==∗
+    txnsys_inv_no_future γ (tail future) ∗
+    ([∗ set] gid ∈ gids_all, group_inv γ gid) ∗
+    ([∗ set] key ∈ keys_all, key_inv γ key) ∗
+    is_txn_committed γ tid wrs.
+  Proof.
+    iIntros (Hhead) "#Htid #Hprep Htxnsys Hgroups Hkeys".
+    do 2 iNamed "Htxnsys".
+    iDestruct (lnrz_tid_elem_of with "Htxnsl Htid") as %Htid.
+    iNamed "Hpart".
+    apply Hfate in Htid as Hcases.
+    destruct Hcases as [Hinresm | Hcases].
+    { (* Case: Txn [tid] has already aborted or committed. *)
+      apply elem_of_dom in Hinresm as [res Hres].
+      destruct res as [wrsc |]; last first.
+      { (* Case: Txn [tid] has already aborted. Contradiction. *)
+        iDestruct (big_sepM_lookup with "Hvr") as "#Hvabt"; first apply Hres.
+        iDestruct (all_prepared_valid_res_aborted with "Hprep Hvabt") as %[].
+      }
+      iDestruct (big_sepM_lookup with "Hvr") as "#Hres"; first apply Hres.
+      iAssert (⌜wrsc = wrs⌝)%I as %->.
+      { iDestruct "Hres" as "[Hwrsc _]".
+        iDestruct "Hprep" as "[Hwrs _]".
+        by iDestruct (txn_wrs_agree with "Hwrs Hwrsc") as %?.
+      }
+      (* Case: Txn [tid] has already committed. Extract a witness without any update. *)
+      iDestruct (txn_res_witness with "Hresm") as "#Hcmt"; first apply Hres.
+      (* Obtain [tid ∉ dom tmodcs] and [tid ∉ dom tmodas]. *)
+      apply lookup_resm_to_tmods_Some in Hres as Hwrs.
+      apply elem_of_dom_2 in Hwrs as Hincmt.
+      iDestruct (big_sepS_elem_of_acc with "Hcmts") as "[Htidexcl HcmtsC]"; first apply Hincmt.
+      iDestruct (excl_tid_not_elem_of with "Hwcmts Htidexcl") as %Hnotinc.
+      iDestruct (excl_tid_not_elem_of with "Hwabts Htidexcl") as %Hnotina.
+      iDestruct ("HcmtsC" with "Htidexcl") as "Hcmts".
+      pose proof (Hcmtxn _ _ Hwrs) as Hinpast. simpl in Hinpast.
+      iDestruct (big_sepL_elem_of with "Hpas") as "Hpawitness"; first apply Hinpast.
+      iCombine "Hpas Hpawitness" as "Hpas'".
+      rewrite -big_sepL_snoc.
+      unshelve epose proof (conflict_free_inv_commit_committed _ _ _ _ _ Hhead Hcf) as Hcf'.
+      { apply not_elem_of_dom_1, Hnotinc. }
+      unshelve epose proof (conflict_past_inv_commit _ _ _ _ _ Hnotina Hhead Hcp) as Hcp'.
+      iDestruct (partitioned_tids_close with "Hwcmts Hwabts Hcmts") as "Hpart".
+      { apply Hfate. }
+      pose proof (cmtxn_in_past_inv_commit_committed _ _ _ _ Hres Hcmtxn) as Hcmtxn'.
+      by iFrame "∗ # %".
+    }
+    destruct Hcases as [Htmodas | Htmodcs].
+    { (* Case: Txn [tid] predicted to abort. Contradiction. *)
+      apply elem_of_dom in Htmodas as Hform.
+      destruct Hform as [form Hform].
+      specialize (Hcp _ _ Hform). simpl in Hcp.
+      rewrite /conflict_cases in Hcp.
+      destruct form as [| | wrsa | wrsa].
+      { (* Case NCA: [tid] not showing at all in [future] -> contradicting [Hhead]. *)
+        destruct (no_commit_head_commit _ _ _ Hcp Hhead) as [].
+      }
+      { (* Case FA: first commit/abort action is abort -> contradicting [Hhead]. *)
+        destruct (first_abort_head_commit _ _ _ Hcp Hhead) as [].
+      }
+      { (* Case FCI: [(tid, wrs)] conflicting with prior action. *)
+        (* Obtain [resm !! ts = None]. *)
+        iDestruct (big_sepS_delete with "Hwabts") as "[Htidexcl Hwabts]"; first apply Htmodas.
+        iDestruct (excl_tid_not_elem_of with "Hcmts Htidexcl") as %Hnotinr.
+        rewrite not_elem_of_dom lookup_resm_to_tmods_None in Hnotinr.
+        destruct Hnotinr as [Hnone | Habt]; last first.
+        { iDestruct (big_sepM_lookup with "Hvr") as "Habt"; first apply Habt.
+          iDestruct (all_prepared_valid_res_aborted with "Hprep Habt") as %[].
+        }
+        (* Obtain [wrsa = wrs] and and incompatible action [a ∈ past]. *)
+        pose proof (first_commit_incompatible_head_commit _ _ _ _ _ Hcp Hhead) as [Heq Hic].
+        subst wrsa.
+        destruct Hic as (a & Hinpast & Hic).
+        (* Take [dom wrs] of [key_inv] and obtain [tid ≠ O]. *)
+        iAssert (⌜dom wrs ⊆ keys_all ∧ tid ≠ O⌝)%I as %[Hdom Htidnz].
+        { iDestruct "Hprep" as "[Hwrs _]".
+          iDestruct (txn_wrs_lookup with "Hwrs Hwrsm") as %Hlookup.
+          apply lookup_wrsm_dbmap_Some in Hlookup.
+          specialize (Hwrsm _ _ Hlookup). simpl in Hwrsm.
+          destruct Hwrsm as [Hvt Hvw].
+          iPureIntro.
+          split; first done.
+          rewrite /valid_ts in Hvt.
+          lia.
+        }
+        iDestruct (big_sepS_subseteq _ _ (dom wrs) with "Hkeys") as "Hkeys".
+        { apply Hdom. }
+        (* Prove that for all [key ∈ dom wrsa], the lock must be currently granted to [tid]. *)
+        iDestruct (keys_inv_prepared_at_ts with "Hprep Hkeys Hresm Hgroups")
+          as "(Hkeys & Hresm & Hgroups)"; first done.
+        iDestruct (big_sepL_elem_of with "Hpas") as "Ha"; first apply Hinpast.
+        destruct a as [tsa wrsa | tsa | tsa keya].
+        { (* Case [a = ActCommit tsa wrsa]. *)
+          apply Decidable.not_or in Hic as [Hge Hne].
+          apply Nat.nlt_ge in Hge.
+          apply set_choose_L in Hne as [k Hk].
+          rewrite elem_of_intersection in Hk.
+          destruct Hk as [Hinwrs Hinwrsa].
+          (* Obtain [tsa < length hlb]. *)
+          simpl.
+          iDestruct (big_sepS_elem_of with "Ha") as (hlb) "[Hhlb %Hlengt]"; first apply Hinwrsa.
+          iDestruct (big_sepS_elem_of with "Hkeys") as "Hkey"; first apply Hinwrs.
+          do 2 iNamed "Hkey".
+          (* Obtain [length hlb ≤ length cmtd]. *)
+          iDestruct (cmtd_hist_prefix with "Hcmtd Hhlb") as %Hprefix.
+          apply prefix_length in Hprefix.
+          (* Obtain [length cmtd ≤ tid]. *)
+          iAssert (⌜(length cmtd ≤ tid)%nat⌝)%I as %Hlenle.
+          { iDestruct (big_sepS_elem_of _ _ k with "Hkmodcs") as "Hkmodc'".
+            { set_solver. }
+            iDestruct (cmtd_kmod_agree with "Hkmodc Hkmodc'") as %Hkmodceq.
+            iPureIntro.
+            eapply ext_by_cmtd_length; [apply Htidnz | | apply Hdiffc].
+            by rewrite -Hkmodceq vslice_resm_to_tmods_not_terminated.
+          }
+          exfalso. clear -Hge Hlengt Hlenle Hprefix. lia.
+        }
+        { (* Case [a = ActAbort tsa]. *)
+          by simpl in Hic.
+        }
+        { (* Case [a = ActRead tsa keya]. *)
+          apply Decidable.not_or in Hic as [Hgt Hin].
+          apply Nat.nle_gt in Hgt.
+          apply dec_stable in Hin.
+          (* Obtain [tsa ≤ length hlb]. *)
+          iDestruct "Ha" as (hlb) "[Hhlb %Hlenge]".
+          (* Obtain [length h ≤ tid]. *)
+          iDestruct (big_sepS_elem_of with "Hkeys") as "Hkey"; first apply Hin.
+          do 2 iNamed "Hkey".
+          (* Obtain [length hlb ≤ length cmtd]. *)
+          iDestruct (cmtd_hist_prefix with "Hcmtd Hhlb") as %Hprefix.
+          apply prefix_length in Hprefix.
+          iAssert (⌜(length cmtd ≤ tid)%nat⌝)%I as %Hlenle.
+          { iDestruct (big_sepS_elem_of _ _ keya with "Hkmodcs") as "Hkmodc'".
+            { set_solver. }
+            iDestruct (cmtd_kmod_agree with "Hkmodc Hkmodc'") as %Hkmodceq.
+            iPureIntro.
+            eapply ext_by_cmtd_length; [apply Htidnz | | apply Hdiffc].
+            by rewrite -Hkmodceq vslice_resm_to_tmods_not_terminated.
+          }
+          exfalso. clear -Hgt Hlenge Hlenle Hprefix. lia.
+        }
+      }
+      { (* Case FCC: [(tid, wrs)] does not satisfy [Q wrs]. *)
+        (* Obtain [wrsa = wrs]. *)
+        destruct Hcp as (lp & ls & Hfc & _).
+        pose proof (first_commit_head_commit _ _ _ _ _ _ Hfc Hhead) as <-.
+        (* Obtain [incorrect_wrs γ tid wrs]. *)
+        iDestruct (big_sepM_lookup with "Hiwrs") as "Hneg"; first apply Hform.
+        simpl.
+        (* Obtain [correct_wrs γ tid wrs]. *)
+        iDestruct "Hprep" as "[Hwrs _]".
+        iDestruct (txn_wrs_lookup with "Hwrs Hwrsm") as %Hwrs.
+        apply lookup_wrsm_dbmap_Some in Hwrs.
+        iDestruct (big_sepM_lookup with "Hcwrs") as "Hpos"; first apply Hwrs.
+        iDestruct (correct_incorrect_wrs with "Hpos Hneg") as %[].
+      }
+    }
+    (* Case: Txn [tid] predicted to commit. Update states and extract commitment witness. *)
+    (* Obtain [resm !! ts = None] and [ts ∉ dom tmodas]. *)
+    iDestruct (big_sepS_delete with "Hwcmts") as "[Htidexcl Hwcmts]"; first apply Htmodcs.
+    iDestruct (excl_tid_not_elem_of with "Hcmts Htidexcl") as %Hnotinr.
+    iDestruct (excl_tid_not_elem_of with "Hwabts Htidexcl") as %Hnotina.
+    rewrite not_elem_of_dom lookup_resm_to_tmods_None in Hnotinr.
+    destruct Hnotinr as [Hnone | Habt]; last first.
+    { iDestruct (big_sepM_lookup with "Hvr") as "Habt"; first apply Habt.
+      iDestruct (all_prepared_valid_res_aborted with "Hprep Habt") as %[].
+    }
+    (* Obtain [wrsx], the write set in the result map of [tid]. *)
+    rewrite elem_of_dom in Htmodcs.
+    destruct Htmodcs as [wrsx Hwrs].
+    (* Obtain eq of write set between the predicted [wrs] and the [wrsx] in the result map. *)
+    pose proof (conflict_free_head_commit_eq _ _ _ _ _ Hcf Hhead Hwrs). subst wrsx.
+    iAssert (⌜dom wrs ⊆ keys_all⌝)%I as %Hdom.
+    { iDestruct "Hprep" as "[Hwrs _]".
+      iDestruct (txn_wrs_lookup with "Hwrs Hwrsm") as %Hlookup.
+      apply lookup_wrsm_dbmap_Some in Hlookup.
+      specialize (Hwrsm _ _ Hlookup).
+      by destruct Hwrsm as [_ Hgoal].
+    }
+    (* Take [dom wrs] of [own_lnrz_kmod_half] and [own_cmtd_kmod_half]. *)
+    iDestruct (big_sepS_subseteq_difference_1 _ _ (dom wrs) with "Hkmodls") as "[Hkmodls HkmodlsO]".
+    { apply Hdom. }
+    iDestruct (big_sepS_subseteq_difference_1 _ _ (dom wrs) with "Hkmodcs") as "[Hkmodcs HkmodcsO]".
+    { apply Hdom. }
+    (* Take [dom wrs] of [key_inv]. *)
+    iDestruct (big_sepS_subseteq_acc _ _ (dom wrs) with "Hkeys") as "[Hkeys HkeysC]".
+    { apply Hdom. }
+    (* Prove that for all [key ∈ dom wrs], the lock must be currently granted to [tid]. *)
+    iDestruct (keys_inv_prepared_at_ts with "Hprep Hkeys Hresm Hgroups")
+      as "(Hkeys & Hresm & Hgroups)"; [done |].
+    (* Extract [own_lnrz_kmod_half] and [own_cmtd_kmod_half] out of [key_inv]. *)
+    iDestruct (keys_inv_with_tsprep_extract_kmodl_kmodc with "Hkeys") as "Hkeys".
+    iDestruct "Hkeys" as (kmodls kmodcs) "(Hkeys & Hkmodls' & Hkmodcs' & %Hdomkmodls)".
+    iDestruct (big_sepM2_dom with "Hkeys") as %Hdomkmodcs.
+    rewrite Hdomkmodls in Hdomkmodcs. symmetry in Hdomkmodcs.
+    (* Agreement of [own_lnrz_kmod_half] and [own_cmtd_kmod_half] from [txnsys_inv] and [key_inv]. *)
+    iDestruct (lnrz_kmod_big_agree with "Hkmodls Hkmodls'") as %Hkmodls.
+    { apply Hdomkmodls. }
+    iDestruct (cmtd_kmod_big_agree with "Hkmodcs Hkmodcs'") as %Hkmodcs.
+    { apply Hdomkmodcs. }
+    (* Agreement and update of [own_lnrz_kmod_half] and [own_cmtd_kmod_half]. *)
+    set tmodcs' := delete tid tmodcs.
+    iMod (lnrz_kmod_big_update (λ k, vslice tmodcs' k) with
+           "Hkmodls Hkmodls'") as "[Hkmodls Hkmodls']".
+    { apply Hdomkmodls. }
+    iAssert ([∗ map] k ↦ kmod ∈ kmodls, own_lnrz_kmod_half γ k (delete tid kmod))%I
+      with "[Hkmodls']" as "Hkmodls'".
+    { iApply (big_sepM_impl with "Hkmodls'").
+      iIntros (k kmod Hkmod) "!> Hkmods".
+      subst tmodcs'.
+      specialize (Hkmodls _ _ Hkmod).
+      by rewrite vslice_delete Hkmodls.
+    }
+    set resm' := <[tid := ResCommitted wrs]> resm.
+    iMod (cmtd_kmod_big_update (λ k, vslice (resm_to_tmods resm') k) with "Hkmodcs Hkmodcs'")
+      as "[Hkmodcs Hkmodcs']".
+    { apply Hdomkmodcs. }
+    iAssert ([∗ map] k ↦ kmod; v ∈ kmodcs; wrs, own_cmtd_kmod_half γ k (<[tid := v]> kmod))%I
+      with "[Hkmodcs']" as "Hkmodcs'".
+    { iApply (big_sepM_sepM2_impl with "Hkmodcs'"); first done.
+      iIntros (k kmod v Hkmod Hv) "!> Hkmods".
+      specialize (Hkmodcs _ _ Hkmod).
+      subst resm'.
+      by rewrite resm_to_tmods_insert_committed (vslice_insert_Some _ _ _ _ _ Hv) Hkmodcs.
+    }
+    (* Prove for each [kmodl] and [kmodc], [is_Some (kmodl !! tid)] and [kmodc !! tid = None]. *)
+    assert (Hkmodlstid : map_Forall (λ _ kmodl, is_Some (kmodl !! tid)) kmodls).
+    { intros k kmodl Hkmodl.
+      specialize (Hkmodls _ _ Hkmodl). simpl in Hkmodls.
+      rewrite Hkmodls lookup_vslice /dual_lookup Hwrs.
+      rewrite -elem_of_dom.
+      apply elem_of_dom_2 in Hkmodl.
+      set_solver.
+    }
+    assert (Hkmodcstid : map_Forall (λ _ kmodc, kmodc !! tid = None) kmodcs).
+    { intros k kmodc Hkmodc.
+      specialize (Hkmodcs _ _ Hkmodc). simpl in Hkmodcs.
+      rewrite Hkmodcs lookup_vslice /dual_lookup.
+      assert (Hresm : resm_to_tmods resm !! tid = None).
+      { rewrite lookup_resm_to_tmods_None. by left. }
+      by rewrite Hresm.
+    }
+    (* Re-establish [key_inv] w.r.t. commit. *)
+    iMod (keys_inv_commit with "Hkeys") as "Hkeys".
+    { by eapply Hnz, elem_of_dom_2. }
+    { intros k kmodl Hkmodl.
+      pose proof (conflict_free_head_commit_le_all _ _ _ _ Hcf Hhead) as Hle.
+      assert (Hk : k ∈ dom wrs).
+      { by rewrite -Hdomkmodls elem_of_dom. }
+      specialize (Hle _ Hk). simpl in Hle.
+      specialize (Hkmodls _ _ Hkmodl). simpl in Hkmodls.
+      by rewrite Hkmodls.
+    }
+    { apply Hkmodlstid. }
+    { apply Hkmodcstid. }
+    rewrite big_sepM2_sep.
+    iDestruct "Hkeys" as "[Hkeys #Hlbs]".
+    rewrite big_sepM2_alt.
+    iDestruct "Hlbs" as "[_ Hlbs]".
+    rewrite -big_sepS_big_sepM dom_map_zip_with_L Hdomkmodls Hdomkmodcs.
+    replace (dom wrs ∩ dom wrs) with (dom wrs); last set_solver.
+    iAssert ([∗ map] k ↦ kmodl;kmodc ∈ kmodls; kmodcs,
+               ∃ v, own_cmtd_kmod_half γ k (<[tid := v]> kmodc) ∗ ⌜kmodl !! tid = Some v⌝)%I
+      with "[Hkmodcs']" as "Hkmodcs'".
+    { rewrite 2!big_sepM2_alt.
+      iDestruct "Hkmodcs'" as "[_ Hkmodcs]".
+      iSplit; first by rewrite Hdomkmodls Hdomkmodcs.
+      iApply (big_sepM_impl_dom_eq with "Hkmodcs").
+      { rewrite 2!dom_map_zip_with_L. set_solver. }
+      iIntros (k kmodcv kmodlc Hkmodcv Hkmodlc) "!> Hkmodcv".
+      destruct kmodcv as [kmodc v]. destruct kmodlc as [kmodl kmodc'].
+      rewrite map_lookup_zip_Some in Hkmodcv. destruct Hkmodcv as [Hkmodc Hv].
+      rewrite map_lookup_zip_Some in Hkmodlc. destruct Hkmodlc as [Hkmodl Hkmodc'].
+      rewrite Hkmodc in Hkmodc'. symmetry in Hkmodc'. inv Hkmodc'.
+      iFrame.
+      iPureIntro.
+      simpl.
+      specialize (Hkmodls _ _ Hkmodl). simpl in Hkmodls.
+      by rewrite Hkmodls lookup_vslice /dual_lookup Hwrs.
+    }
+    iAssert ([∗ set] k ∈ dom wrs, key_inv γ k)%I with "[Hkmodls' Hkmodcs' Hkeys]" as "Hkeys".
+    { iDestruct (big_sepM_big_sepM2_1 _ _ kmodcs with "Hkmodls'") as "Hkmodls'".
+      { by rewrite Hdomkmodls Hdomkmodcs. }
+      iCombine "Hkmodls' Hkmodcs'" as "Hkmods".
+      rewrite -big_sepM2_sep.
+      iCombine "Hkeys Hkmods" as "Hkeys".
+      rewrite -big_sepM2_sep.
+      iApply big_sepS_big_sepM.
+      iApply (big_sepM2_sepM_impl with "Hkeys"); first done.
+      iIntros (k kmodl kmodc v Hkmodl Hkmodc Hv) "!> (Hkey & Hkmodl & Hkmodc)".
+      clear Hv v.
+      iDestruct "Hkmodc" as (v) "[Hkmodc %Hv]".
+      iDestruct "Hkey" as (v') "[Hkey %Hv']".
+      rewrite Hv in Hv'. symmetry in Hv'. inv Hv'.
+      iNamed "Hkey".
+      iFrame "∗ #".
+    }
+    iDestruct ("HkeysC" with "Hkeys") as "Hkeys".
+    (* Update the unmodified part of [own_lnrz_kmod_half]. *)
+    iAssert ([∗ set] x ∈ (keys_all ∖ dom wrs), own_lnrz_kmod_half γ x (vslice tmodcs' x))%I
+      with "[HkmodlsO]" as "HkmodlsO".
+    { iApply (big_sepS_impl with "HkmodlsO").
+      iIntros (k Hk) "!> Hkmod".
+      subst tmodcs'.
+      assert (Hnotinwrs : wrs !! k = None).
+      { rewrite -not_elem_of_dom. set_solver. }
+      by rewrite (vslice_delete_None _ _ _ _ Hwrs Hnotinwrs).
+    }
+    (* Update the unmodified part of [own_cmtd_kmod_half]. *)
+    iAssert ([∗ set] x ∈ (keys_all ∖ dom wrs),
+               own_cmtd_kmod_half γ x (vslice (resm_to_tmods resm') x))%I
+      with "[HkmodcsO]" as "HkmodcsO".
+    { iApply (big_sepS_impl with "HkmodcsO").
+      iIntros (k Hk) "!> Hkmod".
+      subst resm'.
+      rewrite resm_to_tmods_insert_committed.
+      assert (Hnotinwrs : wrs !! k = None).
+      { rewrite -not_elem_of_dom. set_solver. }
+      rewrite (vslice_insert_None _ _ _ _ _ Hnotinwrs); last first.
+      { rewrite lookup_resm_to_tmods_None. by left. }
+      done.
+    }
+    (* Combine the modified and unmodified parts of [own_lnrz_kmod_half] and [own_cmtd_kmod_half]. *)
+    iDestruct (big_sepS_subseteq_difference_2 with "Hkmodls HkmodlsO") as "Hkmodls".
+    { apply Hdom. }
+    iDestruct (big_sepS_subseteq_difference_2 with "Hkmodcs HkmodcsO") as "Hkmodcs".
+    { apply Hdom. }
+    (* Add [(tid, ResCommitted wrs)] to [resm] and extract a witness. *)
+    iMod (txn_res_insert _ (ResCommitted wrs) with "Hresm") as "Hresm"; first apply Hnone.
+    iDestruct (txn_res_witness _ _ tid with "Hresm") as "#Hcmt".
+    { by rewrite lookup_insert. }
+    (* Re-establish [valid_res]. *)
+    iDestruct (big_sepM_insert_2 _ _ tid (ResCommitted wrs) with "[] Hvr") as "Hvr'"; first done.
+    (* Re-establish [past_action_witness]. *)
+    iAssert (past_action_witness γ (ActCommit tid wrs))%I as "#Hpa"; first iFrame "Hlbs".
+    iCombine "Hpas Hpa" as "Hpas'".
+    rewrite -big_sepL_snoc.
+    (* Re-establish [conflict_free], [conflict_past], and [cmtxn_in_past]. *)
+    pose proof (conflict_free_inv_commit _ _ _ _ Hhead Hcf) as Hcf'.
+    pose proof (conflict_past_inv_commit _ _ _ _ _ Hnotina Hhead Hcp) as Hcp'.
+    pose proof (cmtxn_in_past_inv_commit _ _ tid wrs Hcmtxn) as Hcmtxn'.
+    (* Add [tids_excl_frag γ tid] (originally from [wcmts]) to [cmts]. *)
+    iDestruct (big_sepS_insert_2 with "Htidexcl Hcmts") as "Hcmts".
+    iDestruct (partitioned_tids_close tids tmodcs' tmodas resm'
+                with "[Hwcmts] Hwabts [Hcmts]") as "Hpart".
+    { intros tidx Htidx.
+      rewrite dom_insert_L.
+      specialize (Hfate _ Htidx). simpl in Hfate.
+      destruct Hfate as [Hcmt | Hfate].
+      { left. set_solver. }
+      destruct Hfate as [Hwabt | Hwcmt].
+      { right. left. done. }
+      destruct (decide (tidx = tid)) as [-> | Hne].
+      { left. set_solver. }
+      right. right. rewrite dom_delete_L. set_solver.
+    }
+    { by rewrite dom_delete_L. }
+    { by rewrite resm_to_tmods_insert_committed dom_insert_L. }
+    iFrame "∗ # %".
+    iModIntro.
+    iPureIntro.
+    rewrite dom_delete_L.
+    split; last set_solver.
+    intros t m Htm.
+    specialize (Htidcs _ _ Htm). simpl in Htidcs.
+    subst tmodcs' resm'.
+    destruct (decide (t = tid)) as [-> | Hne]; last first.
+    { rewrite lookup_insert_ne; last done.
+      rewrite lookup_delete_ne; last done.
+      apply Htidcs.
+    }
+    right.
+    rewrite lookup_insert.
+    destruct Htidcs as [Hm | Hm].
+    { rewrite Hm in Hwrs. by inv Hwrs. }
+    by rewrite Hm in Hnone.
+  Qed.
+
+End inv.
